Find a way to state hist_bind_resexn_weaken

rupicola/io/RunningExample.fst
@@ -147,18 +147,22 @@ let hist_bind_commut_resexn #a #b (m : hist (resexn a)) (k : a -> io (resexn b))
   end ;
   lem_hist_bind_equiv m m (fun (r : resexn a) -> theta (match r with | Inl x -> k x | Inr x -> io_return (Inr x))) (fun r -> match r with | Inl x -> theta (k x) | Inr x -> hist_return (Inr x))
 
+let hist_inl #a #b (k : a -> hist (resexn b)) (r : resexn a) : hist (resexn b) =
+  fun h lt ->
+    Inl? r ==> k (Inl?.v r) h lt
+
 let hist_bind_resexn_weaken #a #b (m : hist (resexn a)) (k : a -> io (resexn b)) :
   Lemma (
     hist_bind m (fun (r : resexn a) -> theta (match r with | Inl x -> k x | Inr x -> io_return (Inr x))) ⊑
-    hist_bind m (fun r h lt -> Inl? r ==> theta (k (Inl?.v r)) h lt)
+    hist_bind m (hist_inl (fun x -> theta (k x)))
   )
-= (* introduce forall r. (fun (r : resexn a) -> theta (match r with | Inl x -> k x | Inr x -> io_return (Inr x))) r ⊑ (fun r h lt -> Inl? r ==> theta (k (Inl?.v r)) h lt) r
+= introduce forall r. (fun (r : resexn a) -> theta (match r with | Inl x -> k x | Inr x -> io_return (Inr x))) r ⊑ (hist_inl (fun x -> theta (k x))) r
   with begin
-    admit ()
-  end ; *)
-  // assume (forall r. (fun (r : resexn a) -> theta (match r with | Inl x -> k x | Inr x -> io_return (Inr x))) r ⊑ (fun r h lt -> Inl? r ==> theta (k (Inl?.v r)) h lt) r) ;
-  admit () ;
-  lem_hist_bind_subset m m (fun (r : resexn a) -> theta (match r with | Inl x -> k x | Inr x -> io_return (Inr x))) (fun r h lt -> Inl? r ==> theta (k (Inl?.v r)) h lt)
+    match r with
+    | Inl x -> ()
+    | Inr x -> admit ()
+  end ;
+  lem_hist_bind_subset m m (fun (r : resexn a) -> theta (match r with | Inl x -> k x | Inr x -> io_return (Inr x))) (hist_inl (fun x -> theta (k x)))
 
 let read_file_sat_spec f :
   Lemma (theta (read_file f) ⊑ read_file_spec f)
